Integrating

src/asn1/RIoT.Test.fst
@@ -6,18 +6,18 @@ open LowParse.Low.Combinators
 open ASN1.Spec
 open ASN1.Low
 
-module U8 = FStar.UInt8
-module U32 = FStar.UInt32
+// module U8 = FStar.UInt8
+// module U32 = FStar.UInt32
 module HS = FStar.HyperStack
 module HST = FStar.HyperStack.ST
-module MB = LowStar.Monotonic.Buffer
+// module MB = LowStar.Monotonic.Buffer
 module B = LowStar.Buffer
-module Cast = FStar.Int.Cast
+// module Cast = FStar.Int.Cast
 module C = C
 module B32 = FStar.Bytes
 
-open X509.Crypto
-open X509.RIoT
+open X509
+open RIoT.X509
 
 open Lib.IntTypes
 friend Lib.IntTypes
@@ -40,9 +40,8 @@ let sig_t = B.lbuffer uint8 64
 let _ = assert (length_of_oid OID_EC_GRP_SECP256R1 == 6)
 let _ = assert (length_of_asn1_primitive_TLV (Mkbit_string_t 33ul 0ul (magic())) == 35)
 
-
 #restart-solver
-#push-options "--query_stats --z3rlimit 32"
+#push-options "--query_stats --z3rlimit 128 --initial_fuel 8"
 let x509GetAliasCertTBS
   (tbs_len: size_t)
   (tbs: B.lbuffer uint8 (v tbs_len))
@@ -50,8 +49,7 @@ let x509GetAliasCertTBS
   (version: datatype_of_asn1_type INTEGER)
   (aliasKeyPub: key_t)
   (deviceKeyPub: key_t)
-  (fwid_len: asn1_value_int32_of_type OCTET_STRING)
-  (fwid: B.lbuffer uint8 (v fwid_len))
+  (fwid: B.lbuffer uint8 32)
 : HST.StackInline (size_t)
   (requires fun h ->
     B.all_live h [B.buf tbs;
@@ -63,31 +61,57 @@ let x509GetAliasCertTBS
                     B.loc_buffer deviceKeyPub;
                     B.loc_buffer fwid] /\
     0 <= v tbs_pos /\ v tbs_pos <= v tbs_len /\
-    v fwid_len < asn1_length_max - 86 /\
-   (let compositeDeviceID = constructCompositeDeviceID
+   (let compositeDeviceID = x509_get_compositeDeviceID
                             (* version  *) version
                             (* devKeyPub*) (B32.hide (B.as_seq h deviceKeyPub))
-                            (* fwid_len *) fwid_len
                             (* fwid     *) (B32.hide (B.as_seq h fwid)) in
-    let offset = Seq.length (serialize serialize_compositeDeviceID_sequence_TLV compositeDeviceID) in
-    offset <= v tbs_pos))
-  (ensures fun h0 offset h1 ->
-    B.modifies (B.loc_buffer_from_to tbs (tbs_pos -! offset) tbs_pos) h0 h1 (* TODO: refine locs *))
-= let compositeDeviceID = constructCompositeDeviceID
+    let subjectPublicKeyInfo = x509_get_public_key_info
+                               (* alg *) alg_AliasKey
+                               (* pub *) (B32.hide (B.as_seq h aliasKeyPub)) in
+    let offset2 = length_of_opaque_serialization serialize_compositeDeviceID_sequence_TLV compositeDeviceID in
+    let offset1 = length_of_opaque_serialization (serialize_subjectPublicKeyInfo_sequence_TLV alg_AliasKey) subjectPublicKeyInfo in
+    offset1 + offset2 <= v tbs_pos))
+  (ensures fun h0 offset32 h1 ->
+    v offset32 <= v tbs_pos /\
+    B.modifies (B.loc_buffer_from_to tbs (tbs_pos -! offset32) tbs_pos) h0 h1 /\
+   (let compositeDeviceID = x509_get_compositeDeviceID
+                            (* version  *) version
+                            (* devKeyPub*) (B32.hide (B.as_seq h0 deviceKeyPub))
+                            (* fwid     *) (B32.hide (B.as_seq h0 fwid)) in
+    let subjectPublicKeyInfo = x509_get_public_key_info
+                               (* alg *) alg_AliasKey
+                               (* pub *) (B32.hide (B.as_seq h0 aliasKeyPub)) in
+    Seq.slice (B.as_seq h1 tbs) (v tbs_pos - v offset32) (v tbs_pos) ==
+    (serialize_subjectPublicKeyInfo_sequence_TLV alg_AliasKey `serialize` subjectPublicKeyInfo)
+    `Seq.append`
+    (serialize_compositeDeviceID_sequence_TLV `serialize` compositeDeviceID)))
+= let compositeDeviceID = x509_get_compositeDeviceID
                           (* version  *) version
                           (* devKeyPub*) (B32.of_buffer 32ul deviceKeyPub)
-                          (* fwid_len *) fwid_len
-                          (* fwid     *) (B32.of_buffer fwid_len fwid) in
-  let offset = serialize32_compositeDeviceID_TLV_sequence_backwards
-               (* val *) compositeDeviceID
-               (* buf *) tbs
+                          (* fwid     *) (B32.of_buffer 32ul fwid) in
+  let subjectPublicKeyInfo = x509_get_public_key_info
+                             (* alg *) alg_AliasKey
+                             (* pub *) (B32.of_buffer 32ul (aliasKeyPub)) in
+  (* prf *) let h0 = HST.get () in
+  let offset2 = serialize32_compositeDeviceID_sequence_TLV_backwards
+                (* val *) compositeDeviceID
+                 (* buf *) tbs
                (* pos *) tbs_pos in
-  let aliasPubKeyInfo = x509GetAliasKeyInfo (B32.of_buffer 32ul aliasKeyPub) in
-offset
+  (* prf *) let h1 = HST.get () in
+  let offset1 = serialize32_subjectPublicKeyInfo_sequence_TLV_backwards
+                (* alg *) alg_AliasKey
+                (* val *) subjectPublicKeyInfo
+                (* buf *) tbs
+                (* pos *) (tbs_pos -! offset2) in
+  (* prf *) let h2 = HST.get () in
+  (* Prf *) B.modifies_buffer_from_to_elim
+            (* buf *) tbs
+            (*frame*) (tbs_pos -! offset2) (tbs_pos)
+            (* new *) (B.loc_buffer_from_to tbs (tbs_pos -! (offset1 +! offset2)) (tbs_pos -! offset2))
+            (* mem *) h1 (*to*) h2;
+  (* Prf *) Seq.lemma_split (Seq.slice (B.as_seq h2 tbs) (v (tbs_pos -! (offset1 +! offset2))) (v tbs_pos)) (v offset1);
+(* return *) offset1 +! offset2
 #pop-options
-
-let () = ()
-
 
 #restart-solver
 #push-options "--query_stats --z3rlimit 64"
@@ -96,53 +120,18 @@ let main ()
 = HST.push_frame ();
 
   let private_key = B.alloca 0x00uy 32ul in
-  let public_key = Ed25519.secret_to_public private_key in
+  let public_key = P256.secretToPublic private_key in
 
   (* Create TBS region for Alias Key *)
   let buf_len = 500ul in
   let buf = B.alloca 0x00uy buf_len in
-
-  // let algo_oid: b: B.buffer uint8 {B.length b == 2} = B.alloca 0x05uy 2ul in
-  // let algo_param: b: B.buffer uint8 {B.length b == 5} = B.alloca 0x01uy 5ul in
-  // let algo_id: algorithmIdentifier_t = {
-  //   algorithm_oid = (|2ul, B32.of_buffer 2ul algo_oid|);
-  //   parameters    = (|5ul, B32.of_buffer 5ul algo_param|)
-  // } in
-
-  //   (* NOTE: We need to prove this whole constructed SEQUENCE value has a valid length frist. *)
-  // (* Prf *) serialize_algorithmIdentifier_value_unfold algo_id;
-  // (* Prf *) lemma_serialize_asn1_octet_string_TLV_size algo_id.algorithm_oid;
-  // (* Prf *) lemma_serialize_asn1_octet_string_TLV_size algo_id.parameters;
-
-  // (* NOTE: Then reveal the whole constructed SEQUENCE TLV's length. *)
-  // // (* Prf *) serialize_algorithmIdentifier_sequence_unfold algo_id;
-  // (* Prf *) serialize_algorithmIdentifier_sequence_TLV_size algo_id;
-
-  // let pubkey: b: B.buffer uint8 {B.length b == 3} = B.alloca 0b100uy 3ul in
-  // let subjectPublicKeyInfo: subjectPublicKeyInfo_t = {
-  //   algorithm = algo_id;
-  //                      (* FIXME: conflicting with `LowParse.Slice.slice` *)
-  //   subjectPublicKey = Mkbit_string_t 4ul 2ul (B32.of_buffer 3ul pubkey)
-  // } in
-
-  // (* NOTE: Prove subjectPublicKeyInfo is inbound. *)
-  // (* Prf *) serialize_subjectPublicKeyInfo_value_unfold subjectPublicKeyInfo;
-  // (* Prf *) lemma_serialize_asn1_bit_string_TLV_size subjectPublicKeyInfo.subjectPublicKey;
-
-  // (* NOTE: Reveal subjectPublicKeyInfo's TLV's length. *)
-  // (* Prf *) serialize_subjectPublicKeyInfo_sequence_TLV_size subjectPublicKeyInfo;
-
-  // let offset = serialize32_subjectPublicKeyInfo_sequence_TLV_backwards
-  //              (* val *) subjectPublicKeyInfo
-  //              (* buf *) buf
-  //              (* pos *) buf_len in
 
   let offset = 50ul in
 
   let aliasSig = B.alloca 0x00uy 64ul in
   let aliasTBS = B.sub buf (buf_len -! offset) offset in
 
-  Ed25519.sign
+  ECDSA.ecdsa_p256_sha2_sign
     (* sig *) aliasSig
     (* priv*) private_key
     (* len *) offset
