src/asn1/ASN1.Spec.Base.fst
@@ -1,0 +1,25 @@
+module ASN1.Spec.Base
+
+include LowParse.Spec.Base
+include LowParse.Spec.Combinators
+
+unfold
+let coerce_parser_serializer
+  (#t2: Type0)
+  (#k: parser_kind)
+  (#t1: Type0)
+  (#p1: parser k t1)
+  (p2: parser k t2)
+  (s: serializer p1)
+  (u: unit { t2 == t1 /\ p2 == coerce_parser t2 p1} )
+: Tot (serializer (p2))
+= s
+
+unfold
+let length_of_opaque_serialization
+  (#t: Type0)
+  (#k: parser_kind)
+  (#p: parser k t)
+  (s: serializer p)
+  (x: t)
+= Seq.length (s `serialize` x)
