src/asn1/RIoT.Declassify.fsti
@@ -1,0 +1,37 @@
+module RIoT.Declassify
+
+open Lib.IntTypes
+
+module HS = FStar.HyperStack
+module HST = FStar.HyperStack.ST
+module B = LowStar.Buffer
+module C = C
+module B32 = FStar.Bytes
+
+val riot_declassify_public_key
+  (src: B.lbuffer uint8 32)
+  (dst: B.lbuffer pub_uint8 32)
+: HST.Stack unit
+  (requires fun h ->
+    B.live h src /\ B.live h src /\
+    B.disjoint src dst)
+  (ensures fun h0 _ h1 ->
+    B.(modifies (loc_buffer dst) h0 h1) /\
+   (let src_seq = B.as_seq h1 src in
+    let dst_seq = B.as_seq h1 dst in
+    forall (i:nat{0 <= i /\ i < 32}).
+      v (Seq.index dst_seq i) == v (Seq.index src_seq i)))
+
+val riot_declassify_signature
+  (src: B.lbuffer uint8 64)
+  (dst: B.lbuffer pub_uint8 64)
+: HST.Stack unit
+  (requires fun h ->
+    B.live h src /\ B.live h src /\
+    B.disjoint src dst)
+  (ensures fun h0 _ h1 ->
+    B.(modifies (loc_buffer dst) h0 h1) /\
+   (let src_seq = B.as_seq h1 src in
+    let dst_seq = B.as_seq h1 dst in
+    forall (i:nat{0 <= i /\ i < 64}).
+      v (Seq.index dst_seq i) == v (Seq.index src_seq i)))
