src/asn1/RIoT.X509.Base.fst
@@ -1,0 +1,5 @@
+module RIoT.X509.Base
+open X509.Base
+
+let alg_DeviceID = ECDSA_P256
+let alg_AliasKey = ECDSA_P256
