src/asn1/RIoT.X509.CompositeDeviceID.fst
@@ -1,0 +1,196 @@
+module RIoT.X509.CompositeDeviceID
+
+open LowParse.Low.Base
+open LowParse.Low.Combinators
+
+open ASN1.Spec
+open ASN1.Low
+
+open X509.Base
+open X509.BasicFields
+open X509.Crypto
+open RIoT.X509.Base
+open RIoT.X509.FWID
+
+(* CompositeDeviceID *)
+noeq
+type compositeDeviceID_t
+= { riot_version : datatype_of_asn1_type INTEGER;
+    riot_deviceID: subjectPublicKeyInfo_t_inbound alg_DeviceID;
+    riot_fwid    : fwid_t_inbound }
+
+let compositeDeviceID_t'
+= ((datatype_of_asn1_type INTEGER &
+    subjectPublicKeyInfo_t_inbound alg_DeviceID) &
+    fwid_t_inbound)
+
+(* Serialier spec *)
+let synth_compositeDeviceID_t
+  (x': compositeDeviceID_t')
+: GTot (compositeDeviceID_t)
+= { riot_version  = fst (fst x');
+    riot_deviceID = snd (fst x');
+    riot_fwid     = snd x' }
+
+let synth_compositeDeviceID_t'
+  (x: compositeDeviceID_t)
+: Tot (x': compositeDeviceID_t' { x == synth_compositeDeviceID_t x' })
+= ((x.riot_version, x.riot_deviceID), x.riot_fwid)
+
+let parse_compositeDeviceID
+: parser _ (compositeDeviceID_t)
+= parse_asn1_TLV_of_type INTEGER
+  `nondep_then`
+  parse_subjectPublicKeyInfo_sequence_TLV alg_DeviceID
+  `nondep_then`
+  parse_fwid_sequence_TLV
+  `parse_synth`
+  synth_compositeDeviceID_t
+
+let serialize_compositeDeviceID
+: serializer (parse_compositeDeviceID)
+= serialize_synth
+  (* p1 *) (parse_asn1_TLV_of_type INTEGER
+            `nondep_then`
+            parse_subjectPublicKeyInfo_sequence_TLV alg_DeviceID
+            `nondep_then`
+            parse_fwid_sequence_TLV)
+  (* f2 *) (synth_compositeDeviceID_t)
+  (* s1 *) (serialize_asn1_TLV_of_type INTEGER
+            `serialize_nondep_then`
+            serialize_subjectPublicKeyInfo_sequence_TLV alg_DeviceID
+            `serialize_nondep_then`
+            serialize_fwid_sequence_TLV)
+  (* g1 *) (synth_compositeDeviceID_t')
+  (* prf*) ()
+
+let lemma_serialize_compositeDeviceID_unfold
+  (x: compositeDeviceID_t)
+: Lemma (
+  serialize (serialize_compositeDeviceID) x ==
+  serialize (serialize_asn1_TLV_of_type INTEGER) x.riot_version
+  `Seq.append`
+  serialize (serialize_subjectPublicKeyInfo_sequence_TLV alg_DeviceID) x.riot_deviceID
+  `Seq.append`
+  serialize serialize_fwid_sequence_TLV x.riot_fwid
+  // (* unfold subjectPublicKeyInfo *)
+  // serialize (serialize_subjectPublicKeyInfo alg_DeviceID) x.riot_deviceID ==
+  // serialize (serialize_algorithmIdentifier_sequence_TLV alg_DeviceID) x.riot_deviceID.subjectPubKey_alg
+  // `Seq.append`
+  // serialize (serialize_asn1_TLV_of_type BIT_STRING) x.riot_deviceID.subjectPubKey /\
+  // (* unfold FWID *)
+  // serialize serialize_fwid x.riot_fwid ==
+  // serialize (serialize_asn1_TLV_of_type OID) x.riot_fwid.fwid_hashAlg
+  // `Seq.append`
+  // serialize (serialize_asn1_TLV_of_type OCTET_STRING) x.riot_fwid.fwid_value
+)
+= serialize_nondep_then_eq
+  (* s1 *) (serialize_asn1_TLV_of_type INTEGER)
+  (* s2 *) (serialize_subjectPublicKeyInfo_sequence_TLV alg_DeviceID)
+  (* in *) (fst (synth_compositeDeviceID_t' x));
+  serialize_nondep_then_eq
+  (* s1 *) (serialize_asn1_TLV_of_type INTEGER
+            `serialize_nondep_then`
+            serialize_subjectPublicKeyInfo_sequence_TLV alg_DeviceID)
+  (* s2 *) (serialize_fwid_sequence_TLV)
+  (* in *) (synth_compositeDeviceID_t' x);
+  serialize_synth_eq
+  (* p1 *) (parse_asn1_TLV_of_type INTEGER
+            `nondep_then`
+            parse_subjectPublicKeyInfo_sequence_TLV alg_DeviceID
+            `nondep_then`
+            parse_fwid_sequence_TLV)
+  (* f2 *) (synth_compositeDeviceID_t)
+  (* s1 *) (serialize_asn1_TLV_of_type INTEGER
+            `serialize_nondep_then`
+            serialize_subjectPublicKeyInfo_sequence_TLV alg_DeviceID
+            `serialize_nondep_then`
+            serialize_fwid_sequence_TLV)
+  (* g1 *) (synth_compositeDeviceID_t')
+  (* prf*) ()
+  (* in *) x
+    // lemma_serialize_subjectPublicKeyInfo_sequence_TLV_unfold   alg_DeviceID x.riot_deviceID;
+    // lemma_serialize_subjectPublicKeyInfo_unfold                alg_DeviceID x.riot_deviceID;
+    //   lemma_serialize_algorithmIdentifier_sequence_TLV_unfold alg_DeviceID x.riot_deviceID.subjectPubKey_alg;
+    //   lemma_serialize_algorithmIdentifier_sequence_TLV_size   alg_DeviceID x.riot_deviceID.subjectPubKey_alg;
+    // lemma_serialize_fwid_sequence_TLV_unfold x.riot_fwid;
+    // lemma_serialize_fwid_unfold              x.riot_fwid
+
+let lemma_serialize_compositeDeviceID_size
+  (x: compositeDeviceID_t)
+: Lemma (
+  length_of_opaque_serialization (serialize_compositeDeviceID) x ==
+  length_of_asn1_primitive_TLV x.riot_version +
+  length_of_opaque_serialization (serialize_subjectPublicKeyInfo_sequence_TLV alg_DeviceID) x.riot_deviceID +
+  length_of_opaque_serialization serialize_fwid_sequence_TLV x.riot_fwid /\
+  (* subjectPublicKeyInfo size *)
+  length_of_opaque_serialization (serialize_subjectPublicKeyInfo alg_DeviceID) x.riot_deviceID ==
+  length_of_asn1_sequence_TLV (serialize_algorithmIdentifier alg_DeviceID) x.riot_deviceID.subjectPubKey_alg +
+  length_of_asn1_primitive_TLV x.riot_deviceID.subjectPubKey /\
+  (* algorithmIdentifier size*)
+  ( match alg_DeviceID with
+    | ECDSA_P256 -> length_of_opaque_serialization (serialize_algorithmIdentifier alg_DeviceID) x.riot_deviceID.subjectPubKey_alg ==
+                    length_of_asn1_primitive_TLV x.riot_deviceID.subjectPubKey_alg.alg_id_oid_ecdsa +
+                    length_of_asn1_primitive_TLV x.riot_deviceID.subjectPubKey_alg.alg_id_oid_p256 ) /\
+  (* FWID size *)
+  length_of_opaque_serialization serialize_fwid x.riot_fwid ==
+  length_of_asn1_primitive_TLV x.riot_fwid.fwid_hashAlg +
+  length_of_asn1_primitive_TLV x.riot_fwid.fwid_value
+)
+= lemma_serialize_compositeDeviceID_unfold x;
+    lemma_serialize_subjectPublicKeyInfo_sequence_TLV_unfold alg_DeviceID x.riot_deviceID;
+    lemma_serialize_subjectPublicKeyInfo_sequence_TLV_size   alg_DeviceID x.riot_deviceID;
+    lemma_serialize_subjectPublicKeyInfo_unfold              alg_DeviceID x.riot_deviceID;
+    lemma_serialize_subjectPublicKeyInfo_size                alg_DeviceID x.riot_deviceID;
+      lemma_serialize_algorithmIdentifier_sequence_TLV_unfold alg_DeviceID x.riot_deviceID.subjectPubKey_alg;
+      lemma_serialize_algorithmIdentifier_sequence_TLV_size   alg_DeviceID x.riot_deviceID.subjectPubKey_alg;
+      lemma_serialize_algorithmIdentifier_size                alg_DeviceID x.riot_deviceID.subjectPubKey_alg;
+    lemma_serialize_fwid_sequence_TLV_unfold x.riot_fwid;
+    lemma_serialize_fwid_sequence_TLV_size   x.riot_fwid;
+    lemma_serialize_fwid_size                x.riot_fwid
+
+(* inbound sub type*)
+let compositeDeviceID_t_inbound
+= inbound_sequence_value_of (serialize_compositeDeviceID)
+
+(* TLV serializer *)
+let parse_compositeDeviceID_sequence_TLV
+: parser (parse_asn1_envelop_tag_with_TLV_kind SEQUENCE) (compositeDeviceID_t_inbound)
+= compositeDeviceID_t_inbound
+  `coerce_parser`
+  parse_asn1_sequence_TLV (serialize_compositeDeviceID)
+
+let serialize_compositeDeviceID_sequence_TLV
+: serializer (parse_compositeDeviceID_sequence_TLV)
+= coerce_parser_serializer
+  (* t *) (parse_compositeDeviceID_sequence_TLV)
+  (* s *) (serialize_asn1_sequence_TLV (serialize_compositeDeviceID))
+  (*prf*) ()
+
+(* manually unfolding `lemma_serialize_asn1_sequence_TLV_size` to avoid stuck here.  *)
+let lemma_serialize_compositeDeviceID_sequence_TLV_unfold
+= lemma_serialize_asn1_envelop_tag_with_TLV_unfold SEQUENCE (serialize_compositeDeviceID)
+
+let lemma_serialize_compositeDeviceID_sequence_TLV_size
+= lemma_serialize_asn1_sequence_TLV_size (serialize_compositeDeviceID)
+
+let serialize32_compositeDeviceID
+: serializer32_backwards (serialize_compositeDeviceID)
+= serialize32_synth_backwards
+  (* ls *) (serialize32_asn1_TLV_backwards_of_type INTEGER
+            `serialize32_nondep_then_backwards`
+            serialize32_subjectPublicKeyInfo_sequence_TLV_backwards alg_DeviceID
+            `serialize32_nondep_then_backwards`
+            serialize32_fwid_sequence_TLV_backwards)
+  (* f2 *) (synth_compositeDeviceID_t)
+  (* g1 *) (synth_compositeDeviceID_t')
+  (* g1'*) (synth_compositeDeviceID_t')
+  (* prf*) ()
+
+let serialize32_compositeDeviceID_sequence_TLV_backwards
+: serializer32_backwards (serialize_compositeDeviceID_sequence_TLV)
+= coerce_serializer32_backwards
+  (* s2  *) (serialize_compositeDeviceID_sequence_TLV)
+  (* s32 *) (serialize32_asn1_sequence_TLV_backwards
+             (* ls *) (serialize32_compositeDeviceID))
+  (* prf *) ()
