src/asn1/RIoT.X509.FWID.fst
@@ -1,0 +1,123 @@
+module RIoT.X509.FWID
+
+open LowParse.Low.Base
+// open LowParse.Low.Combinators
+
+open ASN1.Spec
+open ASN1.Low
+
+open X509.Crypto
+open X509.BasicFields
+open X509.ExtFields
+
+(* FWID
+  ======
+*)
+noeq
+type fwid_t = {
+  fwid_hashAlg: datatype_of_asn1_type OID; (* OID *)
+  fwid_value  : datatype_of_asn1_type OCTET_STRING
+}
+let fwid_t' = (datatype_of_asn1_type OID & datatype_of_asn1_type OCTET_STRING)
+
+(* Serialier spec *)
+let synth_fwid_t
+  (x': fwid_t')
+: GTot (fwid_t)
+= { fwid_hashAlg = fst x';
+    fwid_value   = snd x' }
+
+let synth_fwid_t'
+  (x: fwid_t)
+: Tot (x': fwid_t' { x == synth_fwid_t x' } )
+= (x.fwid_hashAlg, x.fwid_value)
+
+let parse_fwid
+: parser _ fwid_t
+= parse_asn1_TLV_of_type OID
+  `nondep_then`
+  parse_asn1_TLV_of_type OCTET_STRING
+  `parse_synth`
+  synth_fwid_t
+
+let serialize_fwid
+: serializer parse_fwid
+= serialize_synth
+  (* p1 *) (parse_asn1_TLV_of_type OID
+            `nondep_then`
+            parse_asn1_TLV_of_type OCTET_STRING)
+  (* f2 *) (synth_fwid_t)
+  (* s1 *) (serialize_asn1_TLV_of_type OID
+            `serialize_nondep_then`
+            serialize_asn1_TLV_of_type OCTET_STRING)
+  (* g1 *) (synth_fwid_t')
+  (* prf*) ()
+
+let lemma_serialize_fwid_unfold
+  (x: fwid_t)
+: Lemma (
+  serialize serialize_fwid x ==
+  serialize serialize_asn1_oid_TLV x.fwid_hashAlg
+  `Seq.append`
+  serialize serialize_asn1_octet_string_TLV x.fwid_value
+)
+= serialize_nondep_then_eq
+  (* s1 *) (serialize_asn1_TLV_of_type OID)
+  (* s2 *) (serialize_asn1_TLV_of_type OCTET_STRING)
+  (* in *) (synth_fwid_t' x);
+  serialize_synth_eq
+  (* p1 *) (parse_asn1_TLV_of_type OID
+            `nondep_then`
+            parse_asn1_TLV_of_type OCTET_STRING)
+  (* f2 *) (synth_fwid_t)
+  (* s1 *) (serialize_asn1_TLV_of_type OID
+            `serialize_nondep_then`
+            serialize_asn1_TLV_of_type OCTET_STRING)
+  (* g1 *) (synth_fwid_t')
+  (* prf*) ()
+  (* in *) x
+
+let lemma_serialize_fwid_size
+  (x: fwid_t)
+: Lemma (
+  Seq.length (serialize serialize_fwid x) ==
+  length_of_asn1_primitive_TLV x.fwid_hashAlg +
+  length_of_asn1_primitive_TLV x.fwid_value
+)
+= lemma_serialize_fwid_unfold x
+
+(* inbound sub type*)
+let fwid_t_inbound
+= inbound_sequence_value_of serialize_fwid
+
+(* TLV serializer *)
+let parse_fwid_sequence_TLV
+: parser _ fwid_t_inbound
+= parse_asn1_sequence_TLV serialize_fwid
+
+let serialize_fwid_sequence_TLV
+: serializer parse_fwid_sequence_TLV
+= serialize_asn1_sequence_TLV serialize_fwid
+
+let lemma_serialize_fwid_sequence_TLV_unfold
+= lemma_serialize_asn1_sequence_TLV_unfold serialize_fwid
+
+let lemma_serialize_fwid_sequence_TLV_size
+= lemma_serialize_asn1_sequence_TLV_size serialize_fwid
+
+(* Low *)
+let serialize32_fwid_backwards
+: serializer32_backwards serialize_fwid
+= serialize32_synth_backwards
+  (* ls *) (serialize32_asn1_TLV_backwards_of_type OID
+            `serialize32_nondep_then_backwards`
+            serialize32_asn1_TLV_backwards_of_type OCTET_STRING)
+  (* f2 *) (synth_fwid_t)
+  (* g1 *) (synth_fwid_t')
+  (* g1'*) (synth_fwid_t')
+  (* prf*) ()
+
+let serialize32_fwid_sequence_TLV_backwards
+: serializer32_backwards serialize_fwid_sequence_TLV
+= serialize32_asn1_sequence_TLV_backwards
+  (* ls *) (serialize32_fwid_backwards)
