src/asn1/X509.BasicFields.SubjectPublicKeyInfo.fst
@@ -1,0 +1,150 @@
+module X509.BasicFields.SubjectPublicKeyInfo
+
+open LowParse.Low.Base
+// open LowParse.Low.Combinators
+
+open ASN1.Spec
+open ASN1.Low
+
+open X509.Base
+open X509.Crypto
+
+open FStar.Integers
+
+(* SubjectPublicKeyInfo
+  ======================
+*)
+/// Record repr
+noeq
+type subjectPublicKeyInfo_t
+  (alg: cryptoAlg)
+= { subjectPubKey_alg : algorithmIdentifier_t_inbound alg;
+    subjectPubKey     : datatype_of_asn1_type BIT_STRING }
+
+/// tuple repr
+let subjectPublicKeyInfo_t'
+  (alg: cryptoAlg)
+= tuple2
+  (algorithmIdentifier_t_inbound alg)
+  (datatype_of_asn1_type BIT_STRING)
+
+let synth_subjectPublicKeyInfo_t
+  (alg: cryptoAlg)
+  (x': subjectPublicKeyInfo_t' alg)
+: GTot (subjectPublicKeyInfo_t alg)
+= { subjectPubKey_alg = fst x';
+    subjectPubKey     = snd x' }
+
+let synth_subjectPublicKeyInfo_t'
+  (alg: cryptoAlg)
+  (x: subjectPublicKeyInfo_t alg)
+: Tot (x': subjectPublicKeyInfo_t' alg { x == synth_subjectPublicKeyInfo_t alg x' })
+= (x.subjectPubKey_alg , x.subjectPubKey)
+
+let parse_subjectPublicKeyInfo
+  (alg: cryptoAlg)
+: parser _ (subjectPublicKeyInfo_t alg)
+= parse_algorithmIdentifier_sequence_TLV alg
+  `nondep_then`
+  parse_asn1_TLV_of_type BIT_STRING
+  `parse_synth`
+  synth_subjectPublicKeyInfo_t alg
+
+let serialize_subjectPublicKeyInfo
+  (alg: cryptoAlg)
+: serializer (parse_subjectPublicKeyInfo alg)
+= serialize_synth
+  (* p1 *) (parse_algorithmIdentifier_sequence_TLV alg
+            `nondep_then`
+            parse_asn1_TLV_of_type BIT_STRING)
+  (* f2 *) (synth_subjectPublicKeyInfo_t alg)
+  (* s1 *) (serialize_algorithmIdentifier_sequence_TLV alg
+            `serialize_nondep_then`
+            serialize_asn1_TLV_of_type BIT_STRING)
+  (* g1 *) (synth_subjectPublicKeyInfo_t' alg)
+  (* prf*) ()
+
+let lemma_serialize_subjectPublicKeyInfo_unfold
+  (alg: cryptoAlg)
+  (x: subjectPublicKeyInfo_t alg)
+: Lemma (
+  serialize (serialize_subjectPublicKeyInfo alg) x ==
+  serialize (serialize_algorithmIdentifier_sequence_TLV alg) x.subjectPubKey_alg
+  `Seq.append`
+  serialize (serialize_asn1_TLV_of_type BIT_STRING) x.subjectPubKey
+)
+= serialize_nondep_then_eq
+  (* s1 *) (serialize_algorithmIdentifier_sequence_TLV alg)
+  (* s2 *) (serialize_asn1_TLV_of_type BIT_STRING)
+  (* in *) (synth_subjectPublicKeyInfo_t' alg x);
+  serialize_synth_eq
+  (* p1 *) (parse_algorithmIdentifier_sequence_TLV alg
+            `nondep_then`
+            parse_asn1_TLV_of_type BIT_STRING)
+  (* f2 *) (synth_subjectPublicKeyInfo_t alg)
+  (* s1 *) (serialize_algorithmIdentifier_sequence_TLV alg
+            `serialize_nondep_then`
+            serialize_asn1_TLV_of_type BIT_STRING)
+  (* g1 *) (synth_subjectPublicKeyInfo_t' alg)
+  (* prf*) ()
+  (* in *) x
+
+let lemma_serialize_subjectPublicKeyInfo_size
+  (alg: cryptoAlg)
+  (x: subjectPublicKeyInfo_t alg)
+: Lemma (
+  Seq.length (serialize (serialize_subjectPublicKeyInfo alg) x) ==
+  Seq.length (serialize (serialize_algorithmIdentifier_sequence_TLV alg) x.subjectPubKey_alg) +
+  Seq.length (serialize (serialize_asn1_TLV_of_type BIT_STRING) x.subjectPubKey)
+  // length_of_opaque_serialization (serialize_subjectPublicKeyInfo alg) x ==
+  // length_of_opaque_serialization (serialize_algorithmIdentifier_sequence_TLV alg) x.subjectPubKey_alg +
+  // length_of_opaque_serialization (serialize_asn1_TLV_of_type BIT_STRING) x.subjectPubKey
+)
+= lemma_serialize_subjectPublicKeyInfo_unfold alg x
+
+(* NOTE: Define the `inbound` version of value type after we defined then serializer. *)
+let subjectPublicKeyInfo_t_inbound
+  (alg: cryptoAlg)
+= inbound_sequence_value_of (serialize_subjectPublicKeyInfo alg)
+
+/// TLV
+///
+let parse_subjectPublicKeyInfo_sequence_TLV
+  (alg: cryptoAlg)
+: parser _ (subjectPublicKeyInfo_t_inbound alg)
+= parse_asn1_sequence_TLV (serialize_subjectPublicKeyInfo alg)
+
+let serialize_subjectPublicKeyInfo_sequence_TLV
+  (alg: cryptoAlg)
+: serializer (parse_subjectPublicKeyInfo_sequence_TLV alg)
+= serialize_asn1_sequence_TLV (serialize_subjectPublicKeyInfo alg)
+
+let lemma_serialize_subjectPublicKeyInfo_sequence_TLV_unfold
+  (alg: cryptoAlg)
+= lemma_serialize_asn1_sequence_TLV_unfold (serialize_subjectPublicKeyInfo alg)
+
+let lemma_serialize_subjectPublicKeyInfo_sequence_TLV_size
+  (alg: cryptoAlg)
+= lemma_serialize_asn1_sequence_TLV_size (serialize_subjectPublicKeyInfo alg)
+
+/// Low
+///
+
+inline_for_extraction
+let serialize32_subjectPublicKeyInfo_backwards
+  (alg: cryptoAlg)
+: serializer32_backwards (serialize_subjectPublicKeyInfo alg)
+= serialize32_synth_backwards
+  (* ls *) (serialize32_algorithmIdentifier_sequence_TLV_backwards alg
+            `serialize32_nondep_then_backwards`
+            serialize32_asn1_TLV_backwards_of_type BIT_STRING)
+  (* f2 *) (synth_subjectPublicKeyInfo_t alg)
+  (* g1 *) (synth_subjectPublicKeyInfo_t' alg)
+  (* g1'*) (synth_subjectPublicKeyInfo_t' alg)
+  (* prf*) ()
+
+let serialize32_subjectPublicKeyInfo_sequence_TLV_backwards
+  (alg: cryptoAlg)
+: serializer32_backwards (serialize_subjectPublicKeyInfo_sequence_TLV alg)
+= serialize32_asn1_sequence_TLV_backwards
+  (* ls *) (serialize32_subjectPublicKeyInfo_backwards alg)
