src/asn1/X509.Crypto.AlgorithmIdentifier.fst
@@ -1,0 +1,204 @@
+module X509.Crypto.AlgorithmIdentifier
+
+open LowParse.Low.Base
+// open LowParse.Low.Combinators
+
+open ASN1.Spec
+open ASN1.Low
+
+open X509.Base
+
+open FStar.Integers
+
+(* FIXME: ZT: large structs have bad performance. *)
+
+(* AlgorithmIdentifiers
+  ======================
+  NOTE: Different algorithms have identifiers in different structure.
+*)
+
+(* ECDSA Prime256 SHA2 *)
+noeq
+type algorithmIdentifier_ECDSA_P256_t = {
+  alg_id_oid_ecdsa: oid: datatype_of_asn1_type OID {oid == OID_EC_ALG_UNRESTRICTED};
+  alg_id_oid_p256 : oid: datatype_of_asn1_type OID {oid == OID_EC_GRP_SECP256R1}
+}
+
+let algorithmIdentifier_t
+  (alg: cryptoAlg)
+= match alg with
+  | ECDSA_P256 -> algorithmIdentifier_ECDSA_P256_t
+
+private
+let algorithmIdentifier_t'_aux
+  (alg: cryptoAlg)
+= match alg with
+  | ECDSA_P256 -> tuple2 (datatype_of_asn1_type OID) (datatype_of_asn1_type OID)
+
+/// tuple repr
+let filter_algorithmIdentifier_t'
+  (alg: cryptoAlg)
+  (x': algorithmIdentifier_t'_aux alg)
+: GTot bool
+= match alg with
+  | ECDSA_P256 -> ( let x' = x' <: tuple2 (datatype_of_asn1_type OID) (datatype_of_asn1_type OID) in
+                    fst x' = OID_EC_ALG_UNRESTRICTED &&
+                    snd x' = OID_EC_GRP_SECP256R1 )
+
+let algorithmIdentifier_t'
+  (alg: cryptoAlg)
+= parse_filter_refine (filter_algorithmIdentifier_t' alg)
+
+/// tuple repr -> record repr
+let synth_algorithmIdentifier_t
+  (alg: cryptoAlg)
+  (x': algorithmIdentifier_t' alg)
+: GTot (algorithmIdentifier_t alg)
+= match alg with
+  | ECDSA_P256 -> ( let x' = x' <: tuple2 (datatype_of_asn1_type OID) (datatype_of_asn1_type OID) in
+                    { alg_id_oid_ecdsa = fst x';
+                      alg_id_oid_p256  = snd x' } )
+
+/// record repr -> tuple repr
+let synth_algorithmIdentifier_t'
+  (alg: cryptoAlg)
+  (x: algorithmIdentifier_t alg)
+: Tot (x': algorithmIdentifier_t' alg { x == synth_algorithmIdentifier_t alg x' })
+= match alg with
+  | ECDSA_P256 -> ( let x = x <: algorithmIdentifier_ECDSA_P256_t in
+                    ((x.alg_id_oid_ecdsa <: datatype_of_asn1_type OID),
+                     (x.alg_id_oid_p256  <: datatype_of_asn1_type OID)) )
+
+/// sequence value (body) parser
+let parse_algorithmIdentifier
+  (alg: cryptoAlg)
+: parser _ (algorithmIdentifier_t alg)
+= match alg with
+  | ECDSA_P256 -> ( parse_asn1_TLV_of_type OID
+                    `nondep_then`
+                    parse_asn1_TLV_of_type OID
+                    `parse_filter`
+                    filter_algorithmIdentifier_t' alg
+                    `parse_synth`
+                    synth_algorithmIdentifier_t alg )
+
+/// sequence value serializer
+let serialize_algorithmIdentifier
+  (alg: cryptoAlg)
+: serializer (parse_algorithmIdentifier alg)
+= match alg with
+  | ECDSA_P256 -> ( serialize_synth
+                    (* p1 *) (parse_asn1_TLV_of_type OID
+                              `nondep_then`
+                              parse_asn1_TLV_of_type OID
+                              `parse_filter`
+                              filter_algorithmIdentifier_t' alg)
+                    (* f2 *) (synth_algorithmIdentifier_t alg)
+                    (* s1 *) (serialize_asn1_TLV_of_type OID
+                              `serialize_nondep_then`
+                              serialize_asn1_TLV_of_type OID
+                              `serialize_filter`
+                              filter_algorithmIdentifier_t' alg)
+                    (* g1 *) (synth_algorithmIdentifier_t' alg)
+                    (* prf*) () )
+
+/// lemma: unfold sequence value serializer
+let lemma_serialize_algorithmIdentifier_unfold
+  (alg: cryptoAlg)
+  (x: algorithmIdentifier_t alg)
+: Lemma (
+  match alg with
+  | ECDSA_P256 -> ( serialize (serialize_algorithmIdentifier alg) x ==
+                    serialize (serialize_asn1_TLV_of_type OID) x.alg_id_oid_ecdsa
+                    `Seq.append`
+                    serialize (serialize_asn1_TLV_of_type OID) x.alg_id_oid_p256 ))
+= match alg with
+  | ECDSA_P256 -> ( serialize_nondep_then_eq
+                    (* s1 *) (serialize_asn1_TLV_of_type OID)
+                    (* s2 *) (serialize_asn1_TLV_of_type OID)
+                    (* in *) (synth_algorithmIdentifier_t' alg x);
+                    serialize_synth_eq
+                    (* p1 *) (parse_asn1_TLV_of_type OID
+                              `nondep_then`
+                              parse_asn1_TLV_of_type OID
+                              `parse_filter`
+                              filter_algorithmIdentifier_t' alg)
+                    (* f2 *) (synth_algorithmIdentifier_t alg)
+                    (* s1 *) (serialize_asn1_TLV_of_type OID
+                              `serialize_nondep_then`
+                              serialize_asn1_TLV_of_type OID
+                              `serialize_filter`
+                              filter_algorithmIdentifier_t' alg)
+                    (* g1 *) (synth_algorithmIdentifier_t' alg)
+                    (* prf*) ()
+                    (* in *) x )
+
+/// lemma: reveal sequence serialization size
+let lemma_serialize_algorithmIdentifier_size
+  (alg: cryptoAlg)
+  (x: algorithmIdentifier_t alg)
+: Lemma (
+  match alg with
+  | ECDSA_P256 -> ( Seq.length (serialize (serialize_algorithmIdentifier alg) x) ==
+                    length_of_asn1_primitive_TLV x.alg_id_oid_ecdsa +
+                    length_of_asn1_primitive_TLV x.alg_id_oid_p256 ))
+= match alg with
+  | ECDSA_P256 -> ( lemma_serialize_algorithmIdentifier_unfold alg x )
+
+/// inbound record repr
+let algorithmIdentifier_t_inbound
+  (alg: cryptoAlg)
+= match alg with
+  | ECDSA_P256 -> inbound_sequence_value_of (serialize_algorithmIdentifier alg)
+
+/// TLV
+// unfold
+let parse_algorithmIdentifier_sequence_TLV
+  (alg: cryptoAlg)
+: parser (parse_asn1_envelop_tag_with_TLV_kind SEQUENCE) (algorithmIdentifier_t_inbound alg)
+= match alg with
+  | ECDSA_P256 -> ( algorithmIdentifier_t_inbound alg
+                    `coerce_parser`
+                    parse_asn1_sequence_TLV (serialize_algorithmIdentifier alg) )
+
+let serialize_algorithmIdentifier_sequence_TLV
+  (alg: cryptoAlg)
+: serializer (parse_algorithmIdentifier_sequence_TLV alg)
+= match alg with
+  | ECDSA_P256 -> ( serialize_asn1_sequence_TLV (serialize_algorithmIdentifier alg) )
+
+let lemma_serialize_algorithmIdentifier_sequence_TLV_unfold
+  (alg: cryptoAlg)
+= match alg with
+  | ECDSA_P256 -> ( lemma_serialize_asn1_envelop_tag_with_TLV_size SEQUENCE (serialize_algorithmIdentifier alg) )
+
+let lemma_serialize_algorithmIdentifier_sequence_TLV_size
+  (alg: cryptoAlg)
+= match alg with
+  | ECDSA_P256 -> ( lemma_serialize_asn1_envelop_tag_with_TLV_size SEQUENCE (serialize_algorithmIdentifier alg) )
+
+/// Low
+///
+
+inline_for_extraction
+let serialize32_algorithmIdentifier_backwards
+  (alg: cryptoAlg)
+: serializer32_backwards (serialize_algorithmIdentifier alg)
+= match alg with
+  | ECDSA_P256 -> ( serialize32_synth_backwards
+                    (* ls *) (serialize32_asn1_TLV_backwards_of_type OID
+                              `serialize32_nondep_then_backwards`
+                              serialize32_asn1_TLV_backwards_of_type OID
+                              `serialize32_filter_backwards`
+                              filter_algorithmIdentifier_t' alg)
+                    (* f2 *) (synth_algorithmIdentifier_t alg)
+                    (* g1 *) (synth_algorithmIdentifier_t' alg)
+                    (* g1'*) (synth_algorithmIdentifier_t' alg)
+                    (* prf*) () )
+
+let serialize32_algorithmIdentifier_sequence_TLV_backwards
+  (alg: cryptoAlg)
+: serializer32_backwards (serialize_algorithmIdentifier_sequence_TLV alg)
+= match alg with
+  | ECDSA_P256 -> ( serialize32_asn1_sequence_TLV_backwards
+                    (* s32 *) (serialize32_algorithmIdentifier_backwards alg) )
