src/asn1/X509.Crypto.BigInteger.fst
@@ -1,0 +1,469 @@
+module X509.Crypto.BigInteger
+
+open ASN1.Spec.Base
+open LowParse.Spec.SeqBytes.Base
+
+open ASN1.Base
+open ASN1.Spec.Tag
+open ASN1.Spec.Length
+
+open FStar.Integers
+
+module B32 = FStar.Bytes
+
+unfold
+let big_integer_as_octet_string_t
+= x: datatype_of_asn1_type OCTET_STRING
+  { let (.[]) = B32.index in
+    v (dfst x) > 0 /\                      // no nil
+    ( if (v (dfst x) > 1) then
+      ( B32.index (dsnd x) 0 =!= 0x00uy )  // no leading zero byte if length > 1
+      else ( True ) ) /\
+    ( if ((dsnd x).[0] >= 0x80uy) then   // leave one space for leading zero byte
+      ( v (dfst x) <= asn1_length_max - 7 )
+      else ( True ) ) }
+
+let asn1_value_length_of_big_integer
+= l: asn1_length_t { 0 < l /\ l <= asn1_length_max - 6}
+
+let asn1_value_int32_of_big_integer
+= LowParse.Spec.BoundedInt.bounded_int32 1 (asn1_length_max - 6)
+
+unfold
+let valid_big_integer_as_octet_string_prop
+  (l: asn1_value_length_of_big_integer)
+  (x: big_integer_as_octet_string_t)
+: Type0
+= v (dfst x) > 0 /\
+  ( let (.[]) = B32.index in
+    if l = 1 then
+    ( v (dfst x) == l /\ (dsnd x).[0] < 0x80uy )
+    else if ((dsnd x).[0] >= 0x80uy) then
+    ( v (dfst x) == l - 1 )
+    else
+    ( v (dfst x) == l /\ (dsnd x).[0] > 0x00uy ) )
+
+///
+let filter_big_integer_as_octet_string
+  (l: asn1_value_length_of_big_integer)
+  (s: lbytes l)
+: GTot bool
+= l > 0 &&
+  ( if (l = 1) then
+    ( s.[0] < 0x80uy )
+    else if (s.[0] = 0x00uy) then
+    ( s.[1] >= 0x80uy )
+    else
+    ( s.[0] < 0x80uy ) )
+
+#push-options "--query_stats"
+noextract
+let synth_big_integer_as_octet_string
+  (l: asn1_value_length_of_big_integer)
+  (s: parse_filter_refine (filter_big_integer_as_octet_string l))
+: GTot (value: big_integer_as_octet_string_t
+               { valid_big_integer_as_octet_string_prop l value })
+= if (l = 1) then
+  ( (|1ul, B32.hide s|) )
+  else if (s.[0] = 0x00uy) then
+  ( (|u (l - 1), B32.hide (Seq.slice s 1 l)|) )
+  else
+  ( (|u l, B32.hide s|) )
+
+let lemma_synth_big_integer_as_octet_string_injective'
+  (l: asn1_value_length_of_big_integer)
+  (s s': parse_filter_refine (filter_big_integer_as_octet_string l))
+: Lemma
+  (requires synth_big_integer_as_octet_string l s == synth_big_integer_as_octet_string l s')
+  (ensures s == s')
+= if (l = 1) then
+  ( () )
+  else if (s.[0] = 0x00uy) then
+  ( Seq.lemma_split s  1;
+    Seq.lemma_split s' 1;
+    assert (s `Seq.equal` s') )
+  else
+  ( () )
+
+let lemma_synth_big_integer_as_octet_string_injective
+  (l: asn1_value_length_of_big_integer)
+: Lemma (
+  synth_injective (synth_big_integer_as_octet_string l)
+)
+= synth_injective_intro'
+  (* f *) (synth_big_integer_as_octet_string l)
+  (*prf*) (lemma_synth_big_integer_as_octet_string_injective' l)
+
+/// Encodes our representation of a OCTET_STRING into bytes
+noextract
+let synth_big_integer_as_octet_string_inverse
+  (l: asn1_value_length_of_big_integer)
+  (value: big_integer_as_octet_string_t {valid_big_integer_as_octet_string_prop l value})
+: GTot (s32: parse_filter_refine (filter_big_integer_as_octet_string l)
+            { value == synth_big_integer_as_octet_string l s32 })
+= let (.[]) = B32.index in
+  if l = 1 then
+  ( B32.reveal (dsnd value) )
+  else if (dsnd value).[0] >= 0x80uy then
+  ( let s = Seq.create 1 0x00uy `Seq.append` B32.reveal (dsnd value) in
+    B32.extensionality (dsnd value) (B32.hide (Seq.slice s 1 l));
+    s )
+  else
+  ( B32.reveal (dsnd value) )
+
+// inline_for_extraction noextract
+let parse_big_integer_as_octet_string_kind (l: asn1_value_length_of_big_integer) = constant_size_parser_kind l
+
+///
+/// Parser
+///
+noextract
+let parse_big_integer_as_octet_string
+  (l: asn1_value_length_of_big_integer)
+: parser (parse_big_integer_as_octet_string_kind l) (x: big_integer_as_octet_string_t {valid_big_integer_as_octet_string_prop l x})
+= lemma_synth_big_integer_as_octet_string_injective l;
+  parse_seq_flbytes l
+  `parse_filter`
+  filter_big_integer_as_octet_string l
+  `parse_synth`
+  synth_big_integer_as_octet_string l
+
+///
+/// Serializer
+///
+noextract
+let serialize_big_integer_as_octet_string
+  (l: asn1_value_length_of_big_integer)
+: serializer (parse_big_integer_as_octet_string l)
+= serialize_synth
+  (* p1 *) (parse_seq_flbytes l
+            `parse_filter`
+            filter_big_integer_as_octet_string l)
+  (* f2 *) (synth_big_integer_as_octet_string l)
+  (* s1 *) (serialize_seq_flbytes l
+            `serialize_filter`
+            filter_big_integer_as_octet_string l)
+  (* g1 *) (synth_big_integer_as_octet_string_inverse l)
+  (* Prf*) (lemma_synth_big_integer_as_octet_string_injective l)
+
+///
+/// Lemmas
+///
+
+/// Reveal the computation of serialize
+noextract
+let lemma_serialize_big_integer_as_octet_string_unfold
+  (l: asn1_value_length_of_big_integer)
+  (value: get_parser_type (parse_big_integer_as_octet_string l))
+: Lemma (
+  serialize (serialize_big_integer_as_octet_string l) value ==
+  serialize (serialize_seq_flbytes l) (synth_big_integer_as_octet_string_inverse l value))
+= serialize_synth_eq
+  (* p1 *) (parse_seq_flbytes l
+            `parse_filter`
+            filter_big_integer_as_octet_string l)
+  (* f2 *) (synth_big_integer_as_octet_string l)
+  (* s1 *) (serialize_seq_flbytes l
+            `serialize_filter`
+            filter_big_integer_as_octet_string l)
+  (* g1 *) (synth_big_integer_as_octet_string_inverse l)
+  (* Prf*) (lemma_synth_big_integer_as_octet_string_injective l)
+  (* in *) (value)
+
+/// Reveal the length of a serialzation
+noextract
+let lemma_serialize_big_integer_as_octet_string_size
+  (l: asn1_value_length_of_big_integer)
+  (value: get_parser_type (parse_big_integer_as_octet_string l))
+: Lemma (
+  Seq.length (serialize (serialize_big_integer_as_octet_string l) value) == l)
+= lemma_serialize_big_integer_as_octet_string_unfold l value
+
+
+///////////////////////////////////////////////////////////
+//// ASN1 `OCTET_STRING` TLV Parser and Serializer
+///////////////////////////////////////////////////////////
+
+/// parser tag for the `tagged_union` combinators
+noextract
+let parser_tag_of_big_integer_as_octet_string
+  (x: big_integer_as_octet_string_t)
+: GTot (the_asn1_type INTEGER & asn1_value_int32_of_big_integer)
+= let (.[]) = B32.index in
+  if ((dsnd x).[0] >= 0x80uy) then
+  ( (INTEGER, dfst x + 1ul) )
+  else
+  ( (INTEGER, dfst x) )
+
+open LowParse.Spec.DER
+let parse_asn1_length_kind_of_big_integer
+= parse_bounded_der_length32_kind 1 (asn1_length_max - 6)
+
+let parse_asn1_length_of_big_integer
+= parse_bounded_der_length32 1 (asn1_length_max - 6)
+
+let serialize_asn1_length_of_big_integer
+= serialize_bounded_der_length32 1 (asn1_length_max - 6)
+
+let weak_kind_of_big_integer
+= strong_parser_kind 1 (asn1_length_max - 6) None
+
+inline_for_extraction noextract
+let parse_big_integer_as_octet_string_TLV_kind
+: parser_kind
+= parse_asn1_tag_kind
+  `and_then_kind`
+  parse_asn1_length_kind_of_big_integer
+  `and_then_kind`
+  weak_kind_of_big_integer
+
+noextract
+let synth_big_integer_as_octet_string_V
+  (tag: (the_asn1_type INTEGER & asn1_value_int32_of_big_integer))
+  (value: big_integer_as_octet_string_t
+         { valid_big_integer_as_octet_string_prop (v (snd tag)) value })
+: GTot (refine_with_tag parser_tag_of_big_integer_as_octet_string tag)
+= value
+
+noextract
+let synth_big_integer_as_octet_string_V_inverse
+  (tag: (the_asn1_type INTEGER & asn1_value_int32_of_big_integer))
+  (value': refine_with_tag parser_tag_of_big_integer_as_octet_string tag)
+: GTot (value: big_integer_as_octet_string_t
+               { valid_big_integer_as_octet_string_prop (v (snd tag)) value /\
+                 value' == synth_big_integer_as_octet_string_V tag value})
+= value'
+
+
+///
+/// Aux parser
+///
+noextract
+let parse_big_integer_as_octet_string_V
+  (tag: (the_asn1_type INTEGER & asn1_value_int32_of_big_integer))
+: parser (weak_kind_of_big_integer) (refine_with_tag parser_tag_of_big_integer_as_octet_string tag)
+= weak_kind_of_big_integer
+  `weaken`
+  parse_big_integer_as_octet_string (v (snd tag))
+  `parse_synth`
+  synth_big_integer_as_octet_string_V tag
+
+///
+/// Aux serializer
+///
+noextract
+let serialize_big_integer_as_octet_string_V
+  (tag: (the_asn1_type INTEGER & asn1_value_int32_of_big_integer))
+: serializer (parse_big_integer_as_octet_string_V tag)
+= serialize_synth
+  (* p1 *) (weak_kind_of_big_integer
+            `weaken`
+            parse_big_integer_as_octet_string (v (snd tag)))
+  (* f2 *) (synth_big_integer_as_octet_string_V tag)
+  (* s1 *) (weak_kind_of_big_integer
+            `serialize_weaken`
+            serialize_big_integer_as_octet_string (v (snd tag)))
+  (* g1 *) (synth_big_integer_as_octet_string_V_inverse tag)
+  (* prf*) ()
+
+///
+/// Lemmas
+///
+
+/// Reveal the computation of parse
+noextract
+let lemma_parse_big_integer_as_octet_string_V_unfold
+  (tag: (the_asn1_type INTEGER & asn1_value_int32_of_big_integer))
+  (input: bytes)
+: Lemma (
+  parse (parse_big_integer_as_octet_string_V tag) input ==
+ (match parse (parse_big_integer_as_octet_string (v (snd tag))) input with
+  | None -> None
+  | Some (value, consumed) ->  Some (synth_big_integer_as_octet_string_V tag value, consumed)))
+= parse_synth_eq
+  (* p1 *) (weak_kind_of_big_integer
+            `weaken`
+            parse_big_integer_as_octet_string (v (snd tag)))
+  (* f2 *) (synth_big_integer_as_octet_string_V tag)
+  (* in *) input
+
+/// Reveal the computation of serialzation
+noextract
+let lemma_serialize_big_integer_as_octet_string_V_unfold
+  (tag: (the_asn1_type INTEGER & asn1_value_int32_of_big_integer))
+  (value: refine_with_tag parser_tag_of_big_integer_as_octet_string tag)
+: Lemma (
+  serialize (serialize_big_integer_as_octet_string_V tag) value ==
+  serialize (serialize_big_integer_as_octet_string (v (snd tag))) value
+)
+= serialize_synth_eq
+  (* p1 *) (weak_kind_of_big_integer
+            `weaken`
+            parse_big_integer_as_octet_string (v (snd tag)))
+  (* f2 *) (synth_big_integer_as_octet_string_V tag)
+  (* s1 *) (weak_kind_of_big_integer
+            `serialize_weaken`
+            serialize_big_integer_as_octet_string (v (snd tag)))
+  (* g1 *) (synth_big_integer_as_octet_string_V_inverse tag)
+  (* prf*) ()
+  (* in *) (value)
+
+
+//////////////////////////////////////////////////////////
+
+noextract
+let parse_big_integer_as_octet_string_TLV
+: parser parse_big_integer_as_octet_string_TLV_kind big_integer_as_octet_string_t
+= parse_tagged_union
+  (* pt *) (parse_asn1_tag_of_type INTEGER
+            `nondep_then`
+            parse_asn1_length_of_big_integer)
+  (* tg *) (parser_tag_of_big_integer_as_octet_string)
+  (* p  *) (parse_big_integer_as_octet_string_V)
+
+///
+/// Serializer
+///
+noextract
+let serialize_big_integer_as_octet_string_TLV
+: serializer parse_big_integer_as_octet_string_TLV
+= serialize_tagged_union
+  (* st *) (serialize_asn1_tag_of_type INTEGER
+            `serialize_nondep_then`
+            serialize_asn1_length_of_big_integer)
+  (* tg *) (parser_tag_of_big_integer_as_octet_string)
+  (* s  *) (serialize_big_integer_as_octet_string_V)
+
+///
+/// Lemmas
+///
+
+/// Reveal the computation of serialize
+#push-options "--z3rlimit 32"
+noextract
+let lemma_serialize_big_integer_as_octet_string_TLV_unfold
+  (value: big_integer_as_octet_string_t)
+: Lemma (
+  let tg = parser_tag_of_big_integer_as_octet_string value in
+  serialize serialize_big_integer_as_octet_string_TLV value ==
+  serialize (serialize_asn1_tag_of_type INTEGER) INTEGER
+  `Seq.append`
+  serialize (serialize_asn1_length_of_big_integer) (snd tg)
+  `Seq.append`
+  serialize (serialize_big_integer_as_octet_string (v (snd tg))) value
+)
+= serialize_nondep_then_eq
+  (* s1 *) (serialize_asn1_tag_of_type INTEGER)
+  (* s2 *) (serialize_asn1_length_of_big_integer)
+  (* in *) (parser_tag_of_big_integer_as_octet_string value);
+  lemma_serialize_big_integer_as_octet_string_V_unfold (parser_tag_of_big_integer_as_octet_string value) value;
+  serialize_tagged_union_eq
+  (* st *) (serialize_asn1_tag_of_type INTEGER
+            `serialize_nondep_then`
+            serialize_asn1_length_of_big_integer)
+  (* tg *) (parser_tag_of_big_integer_as_octet_string)
+  (* s  *) (serialize_big_integer_as_octet_string_V)
+  (* in *) (value)
+#pop-options
+
+/// Reveal the size of a serialzation
+#push-options "--z3rlimit 16"
+noextract
+let lemma_serialize_big_integer_as_octet_string_TLV_size
+  (value: big_integer_as_octet_string_t)
+: Lemma (
+  let tg = parser_tag_of_big_integer_as_octet_string value in
+  Seq.length (serialize serialize_big_integer_as_octet_string_TLV value) ==
+  1 + length_of_asn1_length (snd tg) + v (snd tg)
+)
+= let tg = parser_tag_of_big_integer_as_octet_string value in
+  lemma_serialize_big_integer_as_octet_string_TLV_unfold value;
+  lemma_serialize_asn1_tag_of_type_size INTEGER INTEGER;
+  lemma_serialize_asn1_length_size (snd tg);
+  lemma_serialize_asn1_length_unfold (snd tg);
+  serialize_bounded_der_length32_unfold 1 (asn1_length_max - 6) (snd tg);
+  // serialize_asn1_length_of_type_eq INTEGER (dfst value);
+  lemma_serialize_big_integer_as_octet_string_size (v (snd tg)) value
+#pop-options
+
+
+(* Low *)
+
+open ASN1.Low
+module HS = FStar.HyperStack
+module HST = FStar.HyperStack.ST
+module MB = LowStar.Monotonic.Buffer
+module B = LowStar.Buffer
+module Cast = FStar.Int.Cast
+open LowParse.Low.Bytes
+
+#push-options "--query_stats --z3rlimit 32"
+inline_for_extraction
+let serialize32_big_integer_as_octet_string_backwards
+  (len: asn1_value_int32_of_big_integer)
+: Tot (serializer32_backwards (serialize_big_integer_as_octet_string (v len)))
+= fun (x)
+    (#rrel #rel: _)
+    (b: B.mbuffer byte rrel rel)
+    (pos: size_t)
+->  (* prf *) let h0 = HST.get () in
+    (* Prf *) lemma_serialize_big_integer_as_octet_string_unfold (v len) (x);
+    (* Prf *) writable_weaken
+              (* buf *) b
+              (*range*) (v (pos - len)) (v pos)
+              (* mem *) h0
+              (* from*) (v (pos - dfst x))
+              (* to  *) (v pos);
+    store_bytes
+      (* src *) (dsnd x)
+      (* from*) 0ul
+      (* to  *) (dfst x)
+      (* dst *) b
+      (* pos *) (pos - (dfst x));
+
+    if (B32.get (dsnd x) 0ul >= 0x80uy) then
+    ( let h1 = HST.get () in
+      (* Prf *) writable_modifies
+                (* buf *) b
+                (*range*) (v (pos - len)) (v pos)
+                (* mem *) h0
+                (*other*) B.loc_none
+                (* mem'*) h1;
+      (* Prf *) writable_weaken
+                (* buf *) b
+                (*range*) (v (pos - len)) (v pos)
+                (* mem *) h1
+                (* from*) (v (pos - len))
+                (* to  *) (v (pos - dfst x));
+      mbuffer_upd
+        (* buf *) b
+        (*range*) (v (pos - len)) (v pos)
+        (* pos *) (pos - len)
+        (* val *) 0x00uy;
+      (* Prf *) let h2 = HST.get () in
+      (* Prf *) B.modifies_buffer_from_to_elim
+            (* buf *) b
+            (*frame*) (pos - dfst x) (pos)
+            (* new *) (B.loc_buffer_from_to b (pos - len) (pos - dfst x))
+            (* mem *) h1
+            (* mem'*) h2;
+  (* Prf *) Seq.lemma_split (Seq.slice (B.as_seq h2 b) (v (pos - len)) (v pos)) 1 );
+
+(* retuen *) len
+#pop-options
+
+// let serialize32_big_integer_as_octet_string_TLV_backwards ()
+// : Tot (serializer32_backwards (serialize_big_integer_as_octet_string_TLV))
+// = serialize32_tagged_union_backwards
+//   (* lst *) (serialize32_asn1_tag_of_type_backwards INTEGER
+//              `serialize32_nondep_then_backwards`
+//              serialize32_asn1_length_of_type_backwards INTEGER)
+//   (* ltg *) (parser_tag_of_asn1_integer_impl)
+//   (* ls  *) (fun parser_tag -> (serialize32_synth_backwards
+//                               (* ls *) (weak_kind_of_type INTEGER
+//                                         `serialize32_weaken_backwards`
+//                                         serialize32_asn1_integer_backwards (snd parser_tag))
+//                               (* f2 *) (synth_asn1_integer_V parser_tag)
+//                               (* g1 *) (synth_asn1_integer_V_inverse parser_tag)
+//                               (* g1'*) (synth_asn1_integer_V_inverse_impl parser_tag)
+//                               (* prf*) ()))
