src/asn1/X509.Crypto.Signature.fst
@@ -1,0 +1,74 @@
+module X509.Crypto.Signature
+
+open LowParse.Low.Base
+// open LowParse.Low.Combinators
+
+open ASN1.Spec
+open ASN1.Low
+
+open X509.Base
+
+open FStar.Integers
+module B32 = FStar.Bytes
+(*)
+unfold
+let crypto_big_integer_as_octet_string_t
+  (alg: cryptoAlg)
+= match alg with
+  | ECDSA_P256 -> (x: datatype_of_asn1_type OCTET_STRING { v (dfst x) == 32 })
+
+let parse_crypto_big_integer_as_octet_string
+  (alg: cryptoAlg)
+: parser _ (crypto_big_integer_as_octet_string_t alg)
+= match alg with
+  | ECDSA_P256 -> crypto_big_integer_as_octet_string_t ECDSA_P256
+                  `coerce_parser`
+                  parse_asn1_octet_string 32
+
+let serialize_crypto_big_integer_as_octet_string
+  (alg: cryptoAlg)
+: serializer (parse_crypto_big_integer_as_octet_string alg)
+= match alg with
+  | ECDSA_P256 -> coerce_parser_serializer
+                  (* p2 *) (parse_crypto_big_integer_as_octet_string ECDSA_P256)
+                  (* s1 *) (serialize_asn1_octet_string 32)
+                  (* prf*) ()
+open ASN1.Spec.Value.OCTET_STRING
+open ASN1.Spec.Base
+
+let lemma_serialize_crypto_big_integer_as_octet_string_unfold
+  (alg: cryptoAlg)
+= match alg with
+  | ECDSA_P256 -> 
+
+noeq
+type signatureValue_ECDSA_P256_t = {
+  r: B32.lbytes32 32ul;
+  s: B32.lbytes32 32ul
+}
+
+let signatureValue_t
+  (alg: cryptoAlg)
+= match alg with
+  | ECDSA_P256 -> signatureValue_ECDSA_P256_t
+
+let signatureValue_t'
+  (alg: cryptoAlg)
+= match alg with
+  | ECDSA_P256 -> (B32.lbytes32 32ul `tuple2` B32.lbytes32 32ul)
+
+let synth_signatureValue_t
+  (alg: cryptoAlg)
+  (x': signatureValue_t' alg)
+: GTot (signatureValue_t alg)
+= match alg with
+  | ECDSA_P256 -> let r, s = x' <: signatureValue_t' ECDSA_P256 in
+                  {r = r; s = s}
+
+let synth_signatureValue_t'
+  (alg: cryptoAlg)
+  (x: signatureValue_t alg)
+: Tot (x': signatureValue_t' alg { x == synth_signatureValue_t alg x' })
+= match alg with
+  | ECDSA_P256 -> let x = x <: signatureValue_t ECDSA_P256 in
+                  (x.r, x.s)
