src/asn1/X509.RIoT.fst
@@ -1,7 +1,7 @@
 module X509.RIoT
 
 module B32 = FStar.Bytes
-
+(*)
 open ASN1.Spec
 open X509.Crypto
 open X509.RIoT.Ext
